theories/LogicalRelation/Definition/W.v
@@ -1,0 +1,93 @@
+(** * LogRel.LogicalRelation.Definition.Sig : Definition of the logical relation for dependent sums *)
+From Coq Require Import CRelationClasses.
+From LogRel Require Import Utils Syntax.All GenericTyping.
+From LogRel.LogicalRelation.Definition Require Import Prelude Poly.
+
+Set Primitive Projections.
+Set Universe Polymorphism.
+Set Polymorphic Inductive Cumulativity.
+
+
+(** ** Reducibility of dependent sum types *)
+
+Definition WRedTyPack `{ta : tag} `{WfContext ta} `{WfType ta} `{ConvType ta} `{RedType ta} :=
+  ParamRedTyPack (T:=tSig).
+
+Definition SigRedTyAdequate@{i j} `{ta : tag} `{WfContext ta} `{WfType ta} `{ConvType ta} `{RedType ta}
+    {Γ : context} {A B : term} (R : RedRel@{i j}) (ΣA : SigRedTyPack@{i} Γ A B)
+  : Type@{j} := PolyRedPackAdequate R ΣA.
+
+Module SigRedTyPack := ParamRedTyPack.
+
+Inductive isLRPair `{ta : tag} `{WfContext ta}
+  `{WfType ta} `{ConvType ta} `{RedType ta} `{Typing ta} `{ConvTerm ta} `{ConvNeuConv ta}
+  {Γ : context} {A B : term} (ΣA : SigRedTyPack Γ A B) : term -> Type :=
+| PairLRPair : forall (A' B' a b : term)
+      (wtydom : [Γ |- A'])
+      (convtydom : [Γ |- SigRedTyPack.domL ΣA ≅ A'])
+      (wtycod : [Γ |- B'[a..]])
+      (convtycod : [Γ |- (SigRedTyPack.codL ΣA)[a..] ≅ B'[a..]])
+  (rfst : forall {Δ} (ρ : Δ ≤ Γ) (h : [ |- Δ ]),
+      [ΣA.(PolyRedPack.shpRed) ρ h | Δ ||- a⟨ρ⟩ ≅ a⟨ρ⟩ : (SigRedTyPack.domL ΣA)⟨ρ⟩])
+  (rsnd : forall {Δ} (ρ : Δ ≤ Γ) (h : [ |- Δ ]),
+      [ΣA.(PolyRedPack.posRed) ρ h (rfst ρ h) | Δ ||- b⟨ρ⟩ ≅ b⟨ρ⟩ : (SigRedTyPack.codL ΣA)[a⟨ρ⟩ .: (ρ >> tRel)] ]),
+
+  isLRPair ΣA (tPair A' B' a b)
+
+| NeLRPair : forall p : term, [Γ |- p ~ p : SigRedTyPack.outTy ΣA] -> isLRPair ΣA p.
+
+Module SigRedTmEq.
+
+  Record SigRedTm `{ta : tag} `{WfContext ta}
+    `{WfType ta} `{ConvType ta} `{RedType ta}
+    `{Typing ta} `{ConvTerm ta} `{ConvNeuConv ta} `{RedTerm ta}
+    {Γ : context} {A B : term} {ΣA : SigRedTyPack Γ A B} {t : term}
+  : Type := {
+    nf : term;
+    red : [ Γ |- t :⤳*: nf : SigRedTyPack.outTy ΣA ];
+    ispair : isLRPair ΣA nf;
+  }.
+
+  Arguments SigRedTm {_ _ _ _ _ _ _ _ _ _ _ _}.
+
+  Lemma whnf `{GenericTypingProperties} {Γ A B} {ΣA : SigRedTyPack Γ A B} {t} :
+    forall (red : SigRedTm ΣA t), whnf (nf red).
+  Proof.
+    intros [? ? ispair]; simpl; destruct ispair; constructor; tea.
+    now eapply convneu_whne.
+  Qed.
+
+  Definition whred `{GenericTypingProperties} {Γ A B} {ΣA : SigRedTyPack Γ A B} {t} :
+    SigRedTm ΣA t -> [Γ |- t ↘  SigRedTyPack.outTy ΣA].
+  Proof.
+    intros [?? ispair]; econstructor; tea.
+    destruct ispair; constructor; now eapply convneu_whne.
+  Defined.
+
+  Record SigRedTmEq `{ta : tag} `{WfContext ta}
+    `{WfType ta} `{ConvType ta} `{RedType ta}
+    `{Typing ta} `{ConvTerm ta} `{ConvNeuConv ta} `{RedTerm ta}
+    {Γ : context} {A B : term} {ΣA : SigRedTyPack Γ A B} {t u : term}
+  : Type := {
+    redL : SigRedTm ΣA t ;
+    redR : SigRedTm ΣA u ;
+    eq : [ Γ |- redL.(nf) ≅ redR.(nf) : SigRedTyPack.outTy ΣA ];
+    eqFst [Δ] (ρ : Δ ≤ Γ) (h : [ |- Δ ]) :
+      [ΣA.(PolyRedPack.shpRed) ρ h | Δ ||- tFst redL.(nf)⟨ρ⟩ ≅ tFst redR.(nf)⟨ρ⟩ : ΣA.(ParamRedTyPack.domL)⟨ρ⟩] ;
+    eqSnd [Δ] (ρ : Δ ≤ Γ) (h : [ |- Δ ]) :
+      [ΣA.(PolyRedPack.posRed) ρ h (eqFst ρ h) | Δ ||- tSnd redL.(nf)⟨ρ⟩ ≅ tSnd redR.(nf)⟨ρ⟩ : _] ;
+  }.
+
+  Arguments SigRedTmEq {_ _ _ _ _ _ _ _ _ _ _ _}.
+
+  Definition whredL `{GenericTypingProperties} {Γ A B} {ΣA : SigRedTyPack Γ A B} {t u} :
+    SigRedTmEq ΣA t u -> [Γ |- t ↘  SigRedTyPack.outTy ΣA ].
+  Proof. intros []; now eapply whred. Defined.
+
+  Definition whredR `{GenericTypingProperties} {Γ A B} {ΣA : SigRedTyPack Γ A B} {t u} :
+    SigRedTmEq ΣA t u -> [Γ |- u ↘  SigRedTyPack.outTy ΣA ].
+  Proof. intros []; now eapply whred. Defined.
+
+End SigRedTmEq.
+
+Export SigRedTmEq(SigRedTm,Build_SigRedTm, SigRedTmEq,Build_SigRedTmEq).
