theories/Syntax/UntypedReduction.v
@@ -36,8 +36,13 @@ Inductive OneRedAlg : term -> term -> Type :=
 | idElimRefl {A x P hr y A' z} :
   [ tIdElim A x P hr y (tRefl A' z) ⤳ hr ]
 | idElimSubst {A x P hr y e e'} :
-  [e ⤳ e'] ->
+  [ e ⤳ e' ] ->
   [ tIdElim A x P hr y e ⤳ tIdElim A x P hr y e' ]
+| wElimSup {A B P hsup A' B' a k} :
+  [ tWElim A B P hsup (tSup A' B' a k) ⤳ tApp (tApp hsup a) k]
+| wElimSubst {A B P hsup w w'} :
+  [ w ⤳ w' ] ->
+  [ tWElim A B P hsup w ⤳ tWElim A B P hsup w' ]
 
 where "[ t ⤳ t' ]" := (OneRedAlg t t') : typing_scope.
 
@@ -92,7 +97,7 @@ Lemma whnf_nored n u :
 Proof.
   intros nf red.
   induction red in nf |- *.
-  2,3,6,7,9,12: inversion nf; subst; inv_whne; subst; apply IHred; now constructor.
+  2,3,6,7,9,12,14: inversion nf; subst; inv_whne; subst; apply IHred; now constructor.
   all: inversion nf; subst; inv_whne; subst; try now inv_whne.
 Qed.
 
@@ -136,6 +141,11 @@ Proof.
     exfalso; eapply whnf_nored; tea; constructor.
   - inversion red'; subst; try reflexivity.
     exfalso; eapply whnf_nored; tea; constructor.
+  - inversion red'; subst; try reflexivity.
+    exfalso; eapply whnf_nored;tea; constructor.
+  - inversion red'; subst.
+    2: f_equal; eauto.
+    exfalso; eapply whnf_nored;tea; constructor.
   - inversion red'; subst; try reflexivity.
     exfalso; eapply whnf_nored;tea; constructor.
   - inversion red'; subst.
@@ -192,7 +202,7 @@ Lemma oredalg_wk (ρ : nat -> nat) (t u : term) :
 Proof.
   intros Hred.
   induction Hred in ρ |- *.
-  2-12: cbn; rasimpl; now econstructor.
+  2-14: cbn; rasimpl; now econstructor.
   - cbn ; rasimpl.
     evar (t' : term).
     replace (subst_term _ t) with t'.
@@ -258,7 +268,7 @@ induction 1.
   now econstructor.
 Qed.
 
-Lemma redalg_natEmpty {P t t'} : [t ⤳* t'] -> [tEmptyElim P t ⤳* tEmptyElim P t'].
+Lemma redalg_emptyElim {P t t'} : [t ⤳* t'] -> [tEmptyElim P t ⤳* tEmptyElim P t'].
 Proof.
 induction 1.
 + reflexivity.
@@ -279,6 +289,12 @@ Proof.
 Qed.
 
 Lemma redalg_idElim {A x P hr y t t'} : [t ⤳* t'] -> [tIdElim A x P hr y t ⤳* tIdElim A x P hr y t'].
+Proof.
+  induction 1; [reflexivity|].
+  econstructor; tea; now constructor.
+Qed.
+
+Lemma redalg_wElim {A B P hsup t t'} : [t ⤳* t'] -> [tWElim A B P hsup t ⤳* tWElim A B P hsup t'].
 Proof.
   induction 1; [reflexivity|].
   econstructor; tea; now constructor.
